theories/language/neutral_contexts.v
@@ -22,8 +22,10 @@ Class NeutralEctx (k : ectx) := { neutral_ectx : Forall NeutralFrame k }.
 (* ========================================================================== *)
 (** * Instances of Neutral Contexts. *)
 
+#[export]
 Instance EmptyCtx_neutral : NeutralEctx [].
 Proof. by constructor. Qed.
+#[export]
 Instance ConsCtx_neutral f k :
   NeutralFrame f → NeutralEctx k → NeutralEctx (f :: k).
 Proof. constructor. by apply Forall_cons; split; [|apply H0]. Qed.
@@ -32,48 +34,70 @@ Proof. inversion 1. by inversion neutral_ectx0. Qed.
 Lemma ConsCtx_neutral_inv' f k : NeutralEctx (f :: k) → NeutralFrame f.
 Proof. inversion 1. by inversion neutral_ectx0. Qed.
 
+#[export]
 Instance AppLCtx_neutral v2 : NeutralFrame (AppLCtx v2).
 Proof. constructor => m v k σ. by apply AppLEffS. Qed.
+#[export]
 Instance AppRCtx_neutral e1 : NeutralFrame (AppRCtx e1).
 Proof. constructor => m v k σ. by apply AppREffS. Qed.
+#[export]
 Instance DoCtx_neutral m : NeutralFrame (DoCtx m).
 Proof. constructor => m' v k σ. by apply DoEffS. Qed.
+#[export]
 Instance UnOpCtx_neutral op : NeutralFrame (UnOpCtx op).
 Proof. constructor => m v k σ. by apply UnOpEffS. Qed.
+#[export]
 Instance BinOpLCtx_neutral op v2 : NeutralFrame (BinOpLCtx op v2).
 Proof. constructor => m v k σ. by apply BinOpLEffS. Qed.
+#[export]
 Instance BinOpRCtx_neutral op e1 : NeutralFrame (BinOpRCtx op e1).
 Proof. constructor => m v k σ. by apply BinOpREffS. Qed.
+#[export]
 Instance IfCtx_neutral e1 e2 : NeutralFrame (IfCtx e1 e2).
 Proof. constructor => m v k σ. by apply IfEffS. Qed.
+#[export]
 Instance PairLCtx_neutral v2 : NeutralFrame (PairLCtx v2).
 Proof. constructor => m v k σ. by apply PairLEffS. Qed.
+#[export]
 Instance PairRCtx_neutral e1 : NeutralFrame (PairRCtx e1).
 Proof. constructor => m v k σ. by apply PairREffS. Qed.
+#[export]
 Instance FstCtx_neutral : NeutralFrame FstCtx.
 Proof. constructor => m v k σ. by apply FstEffS. Qed.
+#[export]
 Instance SndCtx_neutral : NeutralFrame SndCtx.
 Proof. constructor => m v k σ. by apply SndEffS. Qed.
+#[export]
 Instance InjLCtx_neutral : NeutralFrame InjLCtx.
 Proof. constructor => m v k σ. by apply InjLEffS. Qed.
+#[export]
 Instance InjRCtx_neutral : NeutralFrame InjRCtx.
 Proof. constructor => m v k σ. by apply InjREffS. Qed.
+#[export]
 Instance CaseCtx_neutral e1 e2 : NeutralFrame (CaseCtx e1 e2).
 Proof. constructor => m v k σ. by apply CaseEffS. Qed.
+#[export]
 Instance AllocNLCtx_neutral v2 : NeutralFrame (AllocNLCtx v2).
 Proof. constructor => m v k σ. by apply AllocNLEffS. Qed.
+#[export]
 Instance AllocNRCtx_neutral e1 : NeutralFrame (AllocNRCtx e1).
 Proof. constructor => m v k σ. by apply AllocNREffS. Qed.
+#[export]
 Instance LoadCtx_neutral : NeutralFrame LoadCtx.
 Proof. constructor => m v k σ. by apply LoadEffS. Qed.
+#[export]
 Instance StoreLCtx_neutral v2 : NeutralFrame (StoreLCtx v2).
 Proof. constructor => m v k σ. by apply StoreLEffS. Qed.
+#[export]
 Instance StoreRCtx_neutral e1 : NeutralFrame (StoreRCtx e1).
 Proof. constructor => m v k σ. by apply StoreREffS. Qed.
+#[export]
 Instance CmpXchgLCtx_neutral v2 v3 : NeutralFrame (CmpXchgLCtx v2 v3).
 Proof. constructor => m v k σ. by apply CmpXchgLS. Qed.
+#[export]
 Instance CmpXchgMCtx_neutral e1 v2 : NeutralFrame (CmpXchgMCtx e1 v2).
 Proof. constructor => m v k σ. by apply CmpXchgMS. Qed.
+#[export]
 Instance CmpXchgRCtx_neutral e1 e2 : NeutralFrame (CmpXchgRCtx e1 e2).
 Proof. constructor => m v k σ. by apply CmpXchgRS. Qed.
 
